
> **命题.** $\arctan x + \arctan y = \arctan \frac{x+y}{1-xy}$
>
> 证明：根据 $\tan x$ 和差公式 ，令 $x = \tan \alpha, y = \tan \beta$ ，则得到
>
> $$ \tan(\arctan x + \arctan y) =  \frac{x+y}{1-xy} ,$$
>
> 从而得到 $\arctan x + \arctan y = \arctan \frac{x+y}{1-xy}$。

> **命题.** $\arctan x - \arctan y = \arctan \frac{x-y}{1+xy}$
>
> 证明：根据 $\tan x$ 和差公式 ，令 $x = \tan \alpha, y = \tan \beta$ ，则
>
> $$ \tan(\arctan x - \arctan y) = \frac{x - y}{1+xy}, $$
>
> 从而得到 $\arctan x - \arctan y = \arctan \frac{x-y}{1+xy}$。

> **命题.** $\arctan x + \arctan \frac{1}{x} = \frac{\pi}{2}$
>
> 证明：画个直角三角形，角 $\theta_1$ 对着边长 $1$，$\theta_2 = \frac{\pi}{2} - \theta_1$ 对着边长 $x$，则 $\tan \theta_1 = \frac{1}{x}, \tan \theta_2 = x$，两角互补。



