
$$
  \begin{array}{lllll}
  \text{三角} &  (\tan x)^{\prime} = \sec^2 x & (\cot x)^{\prime} = - \csc^2 x & & \\
                                  & (\sec x)^{\prime} = \sec x \tan x&  (\csc x)^{\prime} = - \csc x \cot x & & \\ 
              &(\sin x)^{(n)} = \sin \left( x + \frac{n\pi}{2} \right)&(\cos x)^{(n)} = \cos \left( x + \frac{n\pi}{2} \right)&&\\
   \text{反三角} & 
                     (\arcsin x)^{\prime} = \frac{1}{\sqrt{1 - x^2}}&
                     (\arccos x)^{\prime} = - \frac{1}{\sqrt{1 - x^2}}& & \\
                    & (\arctan x)^{\prime} = \frac{1}{1 + x^2}&
                                                                (\text{arccot} x)^{\prime} = - \frac{1}{1+x^2} & & \\
   \text{对数三角}&
(\ln |\cos x|)^{\prime} = -\tan x&
                      (\ln |\sin x|)^{\prime} = \cot x& & \\
&                      (\ln |\sec x + \tan x|)^{\prime}  = \sec x&
                                                                  (\ln |\csc x - \cot x|)^{\prime} = \csc x & & \\
    \text{对数根式} &
(\ln (x + \sqrt{x^2 + a^2}))^{\prime} = \frac{1}{\sqrt{x^2 + a^2}}&
    (\ln ( x- \sqrt{x^2 + a^2}))^{\prime} = - \frac{1}{\sqrt{x^2 + a^2}}& & \\
&    (\ln (x + \sqrt{x^2 - a^2}))^{\prime} = \frac{1}{\sqrt{x^2 - a^2}}& 
    (\ln (x - \sqrt{x^2 - a^2}))^{\prime} = - \frac{1}{\sqrt{x^2 - a^2}} & & 
  \end{array}
$$

